concurrency/scache/ClientCounter.i.dfy
@@ -1,0 +1,6 @@
+module ClientCounter {
+  type Client
+
+  glinear method hack_new_client()
+  returns (glinear client: Client)
+}
